Polished solved_form proofs.

hol/redScript.sml
@@ -109,10 +109,11 @@ Cases_on `eq` >> srw_tac [][]);
 val _ = export_rewrites ["FINITE_varseq"];
 
 val solved_form_def = Define`
-  solved_form eqs = FINITE eqs ∧
-  ∀eq. eq ∈ eqs ⇒
-    ∃v t. (eq = (Var v, t)) ∧ (v ∉ vars t) ∧
-          ∀eq'. eq' ∈ eqs ∧ eq' ≠ eq ⇒ v ∉ varseq eq'`;
+  solved_form eqs =
+    FINITE eqs ∧
+    ∀eq. eq ∈ eqs ⇒
+         ∃v t. (eq = (Var v, t)) ∧ (v ∉ vars t) ∧
+               ∀eq'. eq' ∈ eqs ∧ eq' ≠ eq ⇒ v ∉ varseq eq'`;
 
 val FDOM_DISJOINT_vars = Q.store_thm(
 "FDOM_DISJOINT_vars",
@@ -124,40 +125,57 @@ full_simp_tac (srw_ss()) [MEM_MAP,EVERY_MEM,MEM_EL,LIST_EQ_REWRITE] >>
 srw_tac [][rich_listTheory.EL_MAP] >>
 metis_tac []);
 
-val solved_form_unifier = Q.store_thm(
-"solved_form_unifier",
-`solved_form eqs ⇒ (FUN_FMAP (λv. @t. (Var v,t) ∈ eqs) {v | ∃t. (Var v, t) ∈ eqs}) ∈ set_unifier eqs`,
-strip_tac >>
-Q.MATCH_ABBREV_TAC `FUN_FMAP f P ∈ set_unifier eqs` >>
-`P = (IMAGE (term_case I ARB o FST) eqs)` by (
-  srw_tac [][EXTENSION,Abbr`P`,EQ_IMP_THM] >- (
+val eqsvdom_def = Define`eqsvdom eqs = {v | ∃t. (Var v, t) ∈ eqs}`
+
+val FINITE_eqsvdom = store_thm(
+  "FINITE_eqsvdom",
+  ``FINITE eqs ⇒ FINITE (eqsvdom eqs)``,
+  strip_tac >>
+  `eqsvdom eqs ⊆ (IMAGE (term_case I ARB o FST) eqs)` by (
+    srw_tac [][SUBSET_DEF,eqsvdom_def] >- (
     qexists_tac `(Var x, t)` >> srw_tac [][] ) >>
   full_simp_tac (srw_ss()) [solved_form_def] >>
   res_tac >> srw_tac [][] >>
   qexists_tac `t` >> asm_simp_tac pure_ss [] ) >>
+  metis_tac [SUBSET_FINITE, IMAGE_FINITE]);
+
+val solved_form_functional = store_thm(
+  "solved_form_functional",
+  ``solved_form eqs ∧ (v,t1) ∈ eqs ∧ (v,t2) ∈ eqs ⇒ (t1 = t2)``,
+  srw_tac [][solved_form_def] >>
+  first_x_assum (Q.SPEC_THEN `(v,t1)` MP_TAC) >>
+  asm_simp_tac (srw_ss()) [] >>
+  DISCH_THEN (Q.X_CHOOSE_THEN `w` STRIP_ASSUME_TAC) >>
+  first_x_assum (Q.SPEC_THEN `(v,t2)` MP_TAC) >>
+  asm_simp_tac (srw_ss()) []);
+
+val solved_form_unifier = Q.store_thm(
+"solved_form_unifier",
+`solved_form eqs ⇒
+   (FUN_FMAP (λv. @t. (Var v,t) ∈ eqs) (eqsvdom eqs)) ∈ set_unifier eqs`,
+strip_tac >>
+Q.MATCH_ABBREV_TAC `FUN_FMAP f P ∈ set_unifier eqs` >>
 `FINITE eqs` by full_simp_tac pure_ss [solved_form_def] >>
-`FINITE P` by full_simp_tac pure_ss [IMAGE_FINITE] >>
+`FINITE P` by metis_tac [FINITE_eqsvdom] >>
 srw_tac [][set_unifier_def] >>
+`∃v. t1 = Var v` by metis_tac [solved_form_def, PAIR_EQ] >>
+`v ∈ P` by srw_tac [SatisfySimps.SATISFY_ss][Abbr`P`,eqsvdom_def] >>
+srw_tac [][FLOOKUP_FUN_FMAP] >>
+`f v = t2` by (srw_tac [][Abbr`f`] >> SELECT_ELIM_TAC >>
+               metis_tac [solved_form_functional]) >>
+qsuff_tac `DISJOINT (FDOM (FUN_FMAP f P)) (vars t2)`
+  >- metis_tac [FDOM_DISJOINT_vars] >>
+asm_simp_tac (srw_ss())[FUN_FMAP_DEF, DISJOINT_DEF, EXTENSION] >>
+qx_gen_tac `w` >> Cases_on `w ∈ P` >> asm_simp_tac (srw_ss()) [] >>
+`∃t. (Var w,t) ∈ eqs`
+  by full_simp_tac (srw_ss() ++ SatisfySimps.SATISFY_ss)
+                   [Abbr`P`, eqsvdom_def] >>
+`v ∉ vars t2` by metis_tac [solved_form_def, PAIR_EQ, term_11] >>
 full_simp_tac (srw_ss()) [solved_form_def] >>
-UNABBREV_ALL_TAC >>
-res_tac >> srw_tac [][] >>
-srw_tac [][FLOOKUP_FUN_FMAP] >- (
-  SELECT_ELIM_TAC >>
-  srw_tac [][] >- (qexists_tac `t` >> asm_simp_tac pure_ss []) >>
-  res_tac >> srw_tac [][] >>
-  full_simp_tac (srw_ss()) [] >>
-  match_mp_tac (GSYM FDOM_DISJOINT_vars) >>
-  srw_tac [][IN_DISJOINT,FUN_FMAP_DEF] >>
-  Cases_on `x ∈ vars t` >> srw_tac [][] >>
-  Cases_on `x = v` >> full_simp_tac (srw_ss()) [] >>
-  Q.MATCH_ABBREV_TAC `eq ∉ eqs` >>
-  NTAC 2 (FIRST_X_ASSUM (Q.SPEC_THEN `eq` MP_TAC)) >>
-  srw_tac [][Abbr`eq`] >>
-  SPOSE_NOT_THEN STRIP_ASSUME_TAC >>
-  full_simp_tac (srw_ss()) [] >>
-  FIRST_X_ASSUM (Q.SPEC_THEN `(Var v,t)` MP_TAC) >>
-  srw_tac [][] ) >>
-full_simp_tac (srw_ss()) []);
+first_x_assum (Q.SPEC_THEN `(Var w,t)` MP_TAC) >>
+srw_tac [][] >>
+first_x_assum (Q.SPEC_THEN `(Var v,f v)` MP_TAC) >>
+srw_tac [][] >> metis_tac []);
 
 (* prove the solved form unifier most general? *)
 
